src/SymILProofs.v
@@ -17,7 +17,7 @@ Require Import ILEnv SymIL.
 Set Implicit Arguments.
 Set Strict Implicit.
 
-(** The Symbolic Evaluation Interfaces *)
+(** The Symolic Evaluation Interfaces *)
 Module MEVAL := SymIL.MEVAL.
 
 Module SymIL_Correct.
@@ -25,12 +25,12 @@ Module SymIL_Correct.
     Variable ts : list type.
     Let types := repr bedrock_types_r ts.
 
-    Local Notation "'pcT'" := (tvType 0).
-    Local Notation "'tvWord'" := (tvType 0).
-    Local Notation "'stT'" := (tvType 1).
-    Local Notation "'tvState'" := (tvType 2).
-    Local Notation "'tvTest'" := (tvType 3).
-    Local Notation "'tvReg'" := (tvType 4).
+    Notation pcT := (tvType 0).
+    Notation tvWord := (tvType 0).
+    Notation stT := (tvType 1).
+    Notation tvState := (tvType 2).
+    Notation tvTest := (tvType 3).
+    Notation tvReg := (tvType 4).
 
     Variable fs : functions types.
     Let funcs := repr (bedrock_funcs_r ts) fs.
@@ -47,6 +47,17 @@ Module SymIL_Correct.
     Variable meta_env : env types.
     Variable vars_env : env types.
 
+    Lemma stateD_interp : forall cs stn_st ss sh,
+      stateD funcs preds meta_env vars_env cs stn_st ss ->
+      SymMem ss = Some sh ->
+      interp cs (![ MEVAL.SEP.sexprD funcs preds meta_env vars_env (SH.sheapD sh)] stn_st).
+    Proof.
+      clear. destruct stn_st; destruct ss; destruct SymRegs; destruct p; simpl; intros.
+      rewrite H0 in *. intuition.
+    Qed.
+
+    Hint Resolve stateD_interp : sym_eval_hints.
+
     Ltac t_correct := 
       simpl; intros;
         unfold IL_stn_st, IL_mem_satisfies, IL_ReadWord, IL_WriteWord in *;
@@ -58,24 +69,34 @@ Module SymIL_Correct.
                         | Some _ => _
                         | None => _ 
                       end |- _ ] =>
-              revert H; case_eq X; intros; try contradiction
+                revert H; case_eq X; intros; try contradiction
               | [ H : match ?X with 
                         | Some _ => _
                         | None => _ 
                       end = _ |- _ ] =>
-              revert H; case_eq X; intros; try congruence
+                revert H; case_eq X; intros; try congruence
               | [ H : _ = _ |- _ ] => rewrite H
-              | [ H : reg |- _ ] => destruct H
-            end; intuition); subst.
-(*
+              | [ H : @existsEach _ _ _ |- _ ] => apply existsEach_sem in H
+              | [ H : exists x, _ |- _ ] => destruct H
+              | [ H : _ /\ _ |- _ ] => destruct H
+              | [ |- exists x, Some _ = Some _ /\ _ ] =>
+                eexists; split; [ reflexivity | ]
+            end); subst; eauto with sym_eval_hints.
+
     Lemma sym_evalLoc_correct : forall loc ss res res' stn_st locD cs,
       stateD funcs preds meta_env vars_env cs stn_st ss ->
-      sym_locD funcs meta_env vars_env loc = Some locD ->
+      sym_locD fs meta_env vars_env loc = Some locD ->
       evalLoc (snd stn_st) locD = res' ->
       sym_evalLoc loc ss = res -> 
       exprD funcs meta_env vars_env res tvWord = Some res'.
     Proof.
-      destruct loc; unfold stateD; destruct ss; destruct SymRegs; destruct p; subst funcs; t_correct.
+      destruct loc; unfold stateD; destruct ss; destruct SymRegs; destruct p; intros; destruct stn_st; simpl in *;
+        t_correct; try solve [ eauto 
+                             | destruct r; simpl in *; 
+                               repeat match goal with
+                                        | [ H : _ = _ |- _ ] => rewrite H
+                                        | [ |- _ ] => subst funcs
+                                      end; eauto ].
     Qed.
     
     Hypothesis Valid_facts : Valid PC meta_env vars_env facts.
@@ -88,18 +109,15 @@ Module SymIL_Correct.
         evalRvalue (fst stn_st) (snd stn_st) rvD = Some val /\
         exprD funcs meta_env vars_env res tvWord = Some val.
     Proof.
-      destruct rv; unfold stateD; t_correct; try congruence;
-        try solve [ destruct ss; destruct SymRegs; destruct p; intuition; t_correct; eauto ].
-
-      destruct s; t_correct; destruct ss; destruct SymRegs; destruct p; intuition; t_correct; eauto.
-      t_correct;
-      match goal with
-        | [ H : MEVAL.smemeval_read_word _ _ _ _ _ = _ |- _ ] => 
-          eapply (MEVAL.ReadCorrect meval_correct) in H; eauto; t_correct
-      end; eauto.
-      eapply sym_evalLoc_correct with (cs := cs); eauto. instantiate (1 := (s0, s1)). t_correct.
-      reflexivity.
-      congruence.
+      Opaque stateD sym_locD.
+      destruct rv; t_correct. 
+      { destruct s; t_correct. 
+        { erewrite <- (@sym_evalLoc_correct (SymReg _ r)). f_equal. eauto. simpl.
+          Transparent sym_locD. simpl. reflexivity. Opaque sym_locD. reflexivity. reflexivity. }
+        { eapply (MEVAL.ReadCorrect meval_correct) with (cs := cs) in H2; eauto with sym_eval_hints.
+          2: eapply sym_evalLoc_correct; (instantiate; eauto with sym_eval_hints). 2: eauto.
+          t_correct. } }
+      { congruence. }
     Qed.
           
     Lemma sym_evalLval_correct : forall lv stn_st lvD cs val ss ss' valD,
@@ -111,32 +129,33 @@ Module SymIL_Correct.
         evalLvalue (fst stn_st) (snd stn_st) lvD valD = Some st' /\
         stateD funcs preds meta_env vars_env cs (fst stn_st, st') ss'.
     Proof.
-      destruct lv.
-        Focus.
-        destruct ss; destruct SymRegs; destruct p. unfold funcs in *.
-          t_correct; eexists; repeat (split; try reflexivity; eauto);
-            try solve [ repeat rewrite sepFormula_eq in *; unfold sepFormula_def in *; simpl in *; auto ].
-
-        Focus.
-        unfold funcs in *.
-        t_correct.
-        eapply sym_evalLoc_correct with (stn_st := (s0, s1)) in H0; simpl in *; eauto.
-        destruct ss; intuition. destruct SymRegs. destruct p. simpl in *. subst. intuition.
-        repeat match type of H1 with
-                 | match ?X with | Some _ => _ | None => _ end => destruct X; try contradiction
-               end.            
+      destruct lv; t_correct.
+      { Transparent stateD. unfold stateD in *. t_correct. Opaque stateD.
+        case_eq (sym_setReg r val (SymRegs ss)); intros.
+        destruct ss; destruct SymRegs; destruct p. t_correct.
+        unfold sym_setReg in H0. destruct r; inversion H0; subst; t_correct; unfold rupd; simpl; intuition;
+        try solve [ repeat rewrite sepFormula_eq in *; unfold sepFormula_def in *; simpl in *; auto ].
+        destruct r; inversion H0; subst; t_correct; unfold rupd; simpl; intuition. }
+      { eapply (@sym_evalLoc_correct s) in H0; eauto.
+        simpl.
         match goal with
-          | [ H : MEVAL.smemeval_write_word _ _ _ _ _ _ = _ |- _ ] => 
-            eapply (MEVAL.WriteCorrect meval_correct) with (cs := cs) (stn_m := (s0,s1)) in H; eauto
+          | [ H : MEVAL.swrite_word _ _ _ _ _ _ = _ |- _ ] => 
+            eapply (MEVAL.WriteCorrect meval_correct) with (cs := cs) (stn_m := (s0,s1)) in H; eauto with sym_eval_hints
         end.
-        destruct (WriteWord s0 (Mem s1) (evalLoc s1 l) valD); try contradiction.
-        eexists; split; [ reflexivity | ]. intuition.
-
-        generalize SEP.sheapD_pures. unfold SEP.ST.satisfies. intro XXX. 
+        simpl in *.
+        destruct (WriteWord s0 (Mem s1) (evalLoc s1 l) valD); try contradiction. t_correct.
+        Transparent stateD. destruct ss; destruct SymRegs; destruct p. simpl in *. Opaque stateD. intuition. subst.
+        generalize SH.sheapD_pures. unfold SEP.ST.satisfies. intro XXX. 
         rewrite sepFormula_eq in H3. unfold sepFormula_def in H3. simpl in *.
-        specialize (@XXX _ _ _ _ preds _ _ cs meta_env vars_env s3 H3). 
-        apply AllProvable_app' in H5. apply AllProvable_app; intuition auto.
+        specialize (@XXX _ _ _ funcs preds meta_env vars_env cs _ _ _ H3). 
+        apply AllProvable_app' in H6. apply AllProvable_app; intuition auto. }
     Qed.
+
+
+    Ltac think := instantiate; simpl;
+      repeat match goal with
+               | [ H : _ = _ |- _ ] => rewrite H
+             end; eauto.
 
     Lemma sym_evalInstr_correct' : forall instr stn_st instrD cs ss ss',
       stateD funcs preds meta_env vars_env cs stn_st ss ->
@@ -146,22 +165,19 @@ Module SymIL_Correct.
         evalInstr (fst stn_st) (snd stn_st) instrD = Some st' /\
         stateD funcs preds meta_env vars_env cs (fst stn_st, st') ss'.
     Proof.
-      Opaque stateD.
-      destruct instr; unfold funcs in *; t_correct; simpl.
-      eapply sym_evalRval_correct in H1; eauto; simpl in *.
-      destruct H1. intuition.
-      eapply sym_evalLval_correct in H2; eauto; simpl in *.
-      destruct H2. intuition. unfold funcs in *; t_correct; eauto.
-
-      repeat match goal with
-               | [ H : _ |- _ ] => progress fold funcs in H
-               | [ H : exists x, _ |- _ ] => destruct H
-               | [ H : _ /\ _ |- _ ] => destruct H 
-               | [ H : sym_rvalueD _ _ _ _ = _ |- _ ] =>
-                 eapply sym_evalRval_correct in H; eauto
-             end.
-      
-      destruct b; eapply sym_evalLval_correct in H3; eauto; unfold funcs in *; t_correct; eauto.
+      destruct instr; t_correct; simpl;
+        repeat match goal with
+                 | [ H : exists x, _ |- _ ] => destruct H
+                 | [ H : _ /\ _ |- _ ] => destruct H
+                 | [ H : sym_rvalueD _ _ _ _ = _ |- _ ] =>
+                   (eapply sym_evalRval_correct in H; think); [ simpl in * ]
+                 | [ H : sym_lvalueD _ _ _ _ = _ |- _ ] =>
+                   (eapply sym_evalLval_correct in H; think); [ simpl in * ]
+                 | [ H : _ = _ |- _ ] => rewrite H
+                 | [ |- _ ] => progress (simpl in * )
+                 | [ b : binop |- _ ] => 
+                   destruct b; unfold fPlus, fMinus, fMult in *; simpl in *
+               end; t_correct.
     Qed.
 
     Lemma sym_assertTest_correct' : forall cs r rD t l lD ss stn_st,
@@ -183,64 +199,62 @@ Module SymIL_Correct.
           end
       end.
     Proof.
-      unfold sym_assertTest; unfold Structured.evalCond; intros;
+      unfold sym_assertTest, Structured.evalCond; destruct stn_st; simpl in *;
         repeat match goal with
-                 | [ |- context [ sym_evalRval ?A ?B ?F ?X ?Y ] ] =>
-                   case_eq (sym_evalRval A B F X Y); intros
-                 | [ |- match ?X with 
-                          | None => True
-                          | Some _ => True
-                        end ] => destruct X; trivial
-               end.
-      case_eq (sym_evalRval Prover meval facts l ss); 
-        case_eq (sym_evalRval Prover meval facts r ss); intros;
-          try solve [ match goal with
-                        | [ |- match ?X with
-                                 | Some _ => _ | None => _ 
-                               end ] => destruct X; intros
-                      end;
-          repeat match goal with
-                   | [ H : _ = _ |- _ ] => rewrite H
-                   | [ |- context [ match ?X with 
-                                      | true => _ | false => _ 
-                                    end ] ] => destruct X
-                   | [ |- context [ match ?X with 
-                                      | IL.Eq => _ | Ne => _ | IL.Lt => _ | Le => _ 
-                                    end ] ] => destruct X
-                 end; trivial ].
-      repeat match goal with
-               | [ H : sym_rvalueD _ _ _ _ = Some _ |- _ ] =>
-                 generalize H ; eapply sym_evalRval_correct in H; eauto
-               | [ H : exists x, _ |- _ ] => destruct H
-               | [ H : _ /\ _ |- _ ] => destruct H
-               | [ H : _ = _ |- _ ] => rewrite H
-             end. intros.
-      unfold Provable; destruct t;
-        repeat (trivial; simpl;
-          match goal with
-            | [ |- context [ match ?X with
-                               | true => _
-                               | false => _
-                             end ] ] => 
-            case_eq X; intros
-            | [ H : exists x, _ |- _ ] => destruct H
-            | [ H : _ /\ _ |- _ ] => destruct H
-            | [ H : _ = _ |- _ ] => rewrite H
-          end);
-        unfold funcs in *; simpl in *;
-          repeat match goal with 
-                   | [ H : exprD _ _ _ _ _ = _ |- _ ] => rewrite H
-                   | [ H : @eq bool (?F _ _) _ |- _ ] => revert H ; clear ; unfold F ; intros
-                 end; simpl;
-          repeat match goal with
-                   | [ H : match ?X with 
-                             | left _ => _
-                             | right _ => _ 
-                           end = _ |- _ ] => destruct X; try congruence
-                 end;
-      eauto 10 using eq_le, lt_le, le_neq_lt.
+                 | [ H : exists x, _ |- _ ] => destruct H
+                 | [ H : _ /\ _ |- _ ] => destruct H
+                 | [ H : sym_rvalueD _ _ _ _ = _ |- _ ] =>
+                   (eapply sym_evalRval_correct in H; think); [ simpl in * ]
+                 | [ H : sym_lvalueD _ _ _ _ = _ |- _ ] =>
+                   (eapply sym_evalLval_correct in H; think); [ simpl in * ]
+                 | [ H : _ = _ |- _ ] => rewrite H
+                 | [ |- _ ] => progress (simpl in * )
+                 | [ |- context [ evalRvalue ?A ?B ?C ] ] => 
+                   case_eq (evalRvalue A B C); intros
+                 | [ |- context [ evalTest ?A ?B ?C ] ] => 
+                   case_eq (evalTest A B C); intros
+                 | [ b : binop |- _ ] => 
+                   destruct b; unfold fPlus, fMinus, fMult in *; simpl in *
+               end; t_correct; simpl in *;
+      try destruct res;
+       repeat match goal with
+        | [ |- context [ sym_evalRval ?A ?B ?C ?D ?E ] ] =>
+          case_eq (sym_evalRval A B C D E); intros
+               end; auto;
+        unfold Provable; destruct t;
+        repeat match goal with
+                 | [ |- match match ?X with 
+                                | Some _ => match ?Y with _ => _ end 
+                                | _ => _
+                              end with _ => _ end ] =>
+                   (case_eq X; trivial; case_eq Y; trivial); []
+                                   
+                 | [ H : exists x, _ |- _ ] => destruct H
+                 | [ H : _ /\ _ |- _ ] => destruct H
+                 | [ H : sym_rvalueD _ _ _ _ = _ |- _ ] =>
+                   (eapply sym_evalRval_correct in H; think); [ simpl in * ]
+                 | [ H : sym_lvalueD _ _ _ _ = _ |- _ ] =>
+                   (eapply sym_evalLval_correct in H; think); [ simpl in * ]
+                 | [ H : _ = _ |- _ ] => rewrite H
+                 | [ |- _ ] => progress (simpl in * )
+                 | [ |- context [ evalRvalue ?A ?B ?C ] ] => 
+                   case_eq (evalRvalue A B C); intros
+                 | [ |- context [ evalTest ?A ?B ?C ] ] => 
+                   Reflection.consider (evalTest A B C); intros
+                 | [ b : binop |- _ ] => 
+                   destruct b; unfold fPlus, fMinus, fMult in *; simpl in *
+                 | [ |- _ ] => progress t_correct
+               end; unfold IL.weqb, IL.wneb, wltb, wleb in *; simpl in *;
+        repeat match goal with
+                 | [ H : (if ?X then _ else _) = _ |- _ ] =>
+                   revert H; Reflection.consider X; try congruence
+                 | [ H : Some _ = Some _ |- _ ] => inversion H; clear H; subst
+                 | [ H : ?X = _ , H' : ?X = _ |- _ ] => rewrite H in H'
+                 | [ |- context [ wlt_dec ?X ?Y ] ] =>
+                   destruct (wlt_dec X Y); try congruence
+               end; try congruence; eauto 10 using eq_le, lt_le, le_neq_lt.
     Qed.
-*)
+
   End typed.
 
 
@@ -248,12 +262,12 @@ Module SymIL_Correct.
     Variable ts : list type.
     Let types := repr bedrock_types_r ts.
 
-    Local Notation "'pcT'" := (tvType 0).
-    Local Notation "'tvWord'" := (tvType 0).
-    Local Notation "'stT'" := (tvType 1).
-    Local Notation "'tvState'" := (tvType 2).
-    Local Notation "'tvTest'" := (tvType 3).
-    Local Notation "'tvReg'" := (tvType 4).
+    Notation pcT := (tvType 0).
+    Notation tvWord := (tvType 0).
+    Notation stT := (tvType 1).
+    Notation tvState := (tvType 2).
+    Notation tvTest := (tvType 3).
+    Notation tvReg := (tvType 4).
 
     Variable fs : functions types.
     Let funcs := repr (bedrock_funcs_r ts) fs.
@@ -266,7 +280,7 @@ Module SymIL_Correct.
     Variable meval_correct : MEVAL.MemEvaluator_correct meval funcs preds tvWord tvWord
       (@IL_mem_satisfies ts) (@IL_ReadWord ts) (@IL_WriteWord ts).
 
-    Local Ltac t_correct := 
+    Ltac t_correct := 
       simpl; intros;
         unfold IL_stn_st, IL_mem_satisfies, IL_ReadWord, IL_WriteWord in *;
           repeat (simpl in *; 
@@ -317,18 +331,14 @@ Module SymIL_Correct.
             end
         end.
     Proof.
-(*
       Opaque stateD.
       induction is; simpl; intros;
         repeat match goal with
                  | [ H : Some _ = Some _ |- _ ] => inversion H; clear H; subst
                end; simpl; destruct stn_st; simpl in *; eauto.
-
       t_correct. simpl in *.
       case_eq (evalInstr s s0 i); intros.
       case_eq (sym_evalInstr Prover meval facts a ss); intros.      
-
-      Check sym_evalInstr_correct'.
 
       destruct (@sym_evalInstr_correct' ts fs preds Prover PC meval meval_correct facts meta_env var_env
         H a (s,s0) i cs ss s2 H0 H1 H4). simpl in *. intuition.
@@ -347,147 +357,416 @@ Module SymIL_Correct.
         H a (s,s0) i cs ss); eauto.
       simpl in *. destruct H5. rewrite H3 in H5. congruence.
       Transparent stateD.
-*)
-      admit.
     Qed.
 
     Variable learnHook : MEVAL.LearnHook types (SymState types pcT stT).
     Variable learn_correct : @MEVAL.LearnHook_correct _ _ pcT stT learnHook (@stateD _ funcs preds) funcs preds.
 
-    Theorem evalStream_correct : forall sound_or_safe path stn uvars vars st,
-      istreamD funcs uvars vars path stn st sound_or_safe ->
-      forall cs ss,
-        stateD funcs preds uvars vars cs (stn,st) ss ->
-        forall facts, 
-          Valid PC uvars vars facts ->
-          let res := sym_evalStream Prover meval learnHook facts path ss in
-            match res with
-              | inl None => 
-                match sound_or_safe with
-                  | None => True
-                  | Some _ => False
-                end
-              | inl (Some ss') => 
-                match sound_or_safe with
-                  | None => False
-                  | Some st' => 
-                    Expr.forallEach (env_ext (length vars) (SymVars ss')) (fun venv =>
-                      let var_env := vars ++ venv in
-                        Expr.existsEach (env_ext (length uvars) (SymUVars ss')) (fun uenv' =>
-                          let meta_env := uvars ++ uenv' in 
-                            stateD funcs preds meta_env var_env cs (stn, st') ss'))
-                end
-              | inr (ss'', is') => 
-                exists st'' : state, 
-                  Expr.forallEach (env_ext (length vars) (SymVars ss'')) (fun venv =>
-                    let var_env := vars ++ venv in
-                      Expr.existsEach (env_ext (length uvars) (SymUVars ss'')) (fun uenv' =>
-                        let meta_env := uvars ++ uenv' in 
-                          istreamD funcs meta_env var_env is' stn st'' None
-                          /\ stateD funcs preds meta_env var_env cs (stn, st'') ss''))
-            end.
+    Ltac shatter_state ss :=
+      destruct ss as [ ? [ [ ? ? ] ? ] ].
+
+    Lemma skip_to_nil : forall T U (F : T -> U) vars env X,
+      map F env = skipn (length vars) X ->
+      map F nil = skipn (length (vars ++ env)) X.
     Proof.
-      revert learn_correct; revert PC; revert meval_correct. admit.
-(*
-    Opaque stateD.
-    induction path; simpl; intros;
+      clear. induction vars; simpl; intros; subst.
+      induction env; eauto.
+      destruct X; auto.
+    Qed.
+    Lemma AllProvable_cons : forall U G P Ps,
+      Provable funcs U G P ->
+      AllProvable funcs U G Ps ->
+      AllProvable funcs U G (P :: Ps).
+    Proof. simpl; intuition. Qed.
+    Lemma AllProvable_nil : forall U G,
+      AllProvable funcs U G nil.
+    Proof. simpl; intuition. Qed.
+    Hint Resolve AllProvable_cons AllProvable_nil : env_resolution.
+    Hint Resolve Learn_correct : env_resolution.
+    Hint Resolve skip_to_nil : env_resolution.
+
+    Lemma skip_prove_nil : forall T U (F : T -> U) vars env X Y,
+      map F env = skipn (length vars) X ->
+      map F Y = skipn (length (vars ++ env)) X ->
+      Y = nil.
+    Proof.
+      clear. intros. destruct Y; auto.
+      eapply skip_to_nil in H. rewrite <- H in H0. simpl in *; congruence.
+    Qed.
+    Hint Resolve skip_prove_nil : env_resolution.
+    Lemma stateD_addToPures : forall U G cs ss stn_st P,
+      stateD funcs preds U G cs stn_st ss ->
+      Provable funcs U G P ->
+      stateD funcs preds U G cs stn_st 
+      {| SymMem := SymMem ss
+        ; SymRegs := SymRegs ss 
+        ; SymPures := P :: SymPures ss |}.
+    Proof.
+      Transparent stateD.
+      clear. intros; shatter_state ss; destruct stn_st; simpl in *. intuition.
+      destruct SymMem; intuition.
+      Opaque stateD.
+    Qed.
+    Hint Resolve stateD_addToPures : stateD_solver.
+
+    Ltac qstateD_solver :=
+      eapply existsEach_sem; intros; eexists; split; [ solve [ eauto with env_resolution ] | ];
+      let e := fresh in
+      eapply forallEach_sem; intro e; intro;
+      eauto with stateD_solver.
+
+    Opaque repr stateD.
+    Ltac split_congruence := 
+      repeat match goal with 
+               | [ H : prod _ _ |- _ ] => destruct H
+             end; congruence.
+
+    Lemma stateD_weaken_vars : forall uvars vars cs stn_st ss' env,
+      stateD funcs preds uvars vars cs stn_st ss' ->
+      stateD funcs preds uvars (vars ++ env) cs stn_st ss'.
+    Proof.
+      Transparent stateD.
+      clear. intros. destruct stn_st; shatter_state ss'; simpl in *.
       repeat match goal with
+               | [ H : _ /\ _ |- _ ] => destruct H
+               | [ H : context [ match exprD ?A ?B ?C ?D ?E with _ => _ end ] |- _ ] =>
+                 revert H; case_eq (exprD A B C D E); intros; try contradiction
+             end; subst.
+      rewrite <- app_nil_r with (l := uvars). repeat erewrite exprD_weaken by eassumption.
+      intuition. destruct SymMem; auto. erewrite SH.SE_FACTS.sexprD_weaken in H0. eassumption.
+      eapply AllProvable_weaken; eauto. 
+    Qed.
+    Lemma stateD_weaken_uvars : forall uvars vars cs stn_st ss' env,
+      stateD funcs preds uvars vars cs stn_st ss' ->
+      stateD funcs preds (uvars ++ env) vars cs stn_st ss'.
+    Proof.
+      Transparent stateD.
+      clear. intros. destruct stn_st; shatter_state ss'; simpl in *.
+      repeat match goal with
+               | [ H : _ /\ _ |- _ ] => destruct H
+               | [ H : context [ match exprD ?A ?B ?C ?D ?E with _ => _ end ] |- _ ] =>
+                 revert H; case_eq (exprD A B C D E); intros; try contradiction
+             end; subst.
+      rewrite <- app_nil_r with (l := vars). repeat erewrite exprD_weaken by eassumption.
+      intuition. destruct SymMem; auto. erewrite SH.SE_FACTS.sexprD_weaken in H0. eassumption.
+      eapply AllProvable_weaken; eauto. 
+    Qed.
+    Hint Resolve stateD_weaken_vars stateD_weaken_uvars : stateD_solver.
+    Require ListFacts.
+    Require Import Tactics Reflection.
+    Hint Resolve ListFacts.not_sure ListFacts.map_skipn_all_map_is_nil ListFacts.map_skipn_all_map : env_resolution.
+
+    Lemma sym_locD_weaken : forall ts X A C Y Z,
+      sym_locD (types' := ts) X A C Y = Some Z ->
+      forall B D,
+        sym_locD X (A ++ B) (C ++ D) Y = Some Z.
+    Proof.
+      clear. destruct Y; simpl; intros; think; auto; 
+      erewrite exprD_weaken; eauto.
+    Qed.
+
+    Lemma sym_lvalueD_weaken : forall ts X A C Y Z,
+      sym_lvalueD (types' := ts) X A C Y = Some Z ->
+      forall B D,
+        sym_lvalueD X (A ++ B) (C ++ D) Y = Some Z.
+    Proof.
+      clear. destruct Y; simpl; intros; think; auto.
+      erewrite sym_locD_weaken; eauto.
+    Qed.      
+    Lemma sym_rvalueD_weaken : forall ts X A C Y Z,
+      sym_rvalueD (types' := ts) X A C Y = Some Z ->
+      forall B D,
+        sym_rvalueD X (A ++ B) (C ++ D) Y = Some Z.
+    Proof.
+      clear. destruct Y; simpl; intros; think; auto.
+      erewrite sym_lvalueD_weaken; eauto.
+      erewrite exprD_weaken; eauto.
+    Qed.
+
+    Lemma sym_instrD_weaken : forall ts X A C Y Z,
+      sym_instrD (types' := ts) X A C Y = Some Z ->
+      forall B D,
+      sym_instrD X (A ++ B) (C ++ D) Y = Some Z.
+    Proof.
+      clear; destruct Y; simpl; intros; think; auto;
+        repeat ((erewrite sym_lvalueD_weaken by eauto) ||
+                (erewrite sym_rvalueD_weaken by eauto)); auto.
+    Qed.
+
+    Lemma sym_instrsD_weaken : forall ts X A C Y Z,
+      sym_instrsD (types' := ts) X A C Y = Some Z ->
+      forall B D,
+      sym_instrsD X (A ++ B) (C ++ D) Y = Some Z.
+    Proof.
+      clear. induction Y; simpl; intros; think; auto.
+      erewrite sym_instrD_weaken; eauto.
+    Qed.
+
+    Lemma istreamD_weaken : forall ts X A C Y Z P L,
+      istreamD (types' := ts) X A C Y Z P L ->
+      forall B D,
+      istreamD X (A ++ B) (C ++ D) Y Z P L.
+    Proof.
+      clear. induction Y; simpl; intros; think; auto.
+      repeat match goal with 
+               | [ H : match ?X with _ => _ end |- _ ] =>
+                 consider X; intros
+               | [ H : _ /\ _ |- _ ] => destruct H
+               | [ |- _ ] =>
+                 (erewrite sym_instrsD_weaken by eauto) ||
+                 (erewrite sym_rvalueD_weaken by eauto) ||
+                 (erewrite sym_lvalueD_weaken by eauto)
+             end; intuition.
+    Qed.
+
+    Lemma env_nil_by_length_eq : forall ts L X Y,
+      typeof_env (types := ts) L = X ->
+      length Y = length X ->
+      typeof_env (types := ts) nil = skipn (length L) Y.
+    Proof.
+      clear. intros. subst.
+      erewrite ListFacts.skipn_length_gt; auto. unfold typeof_env in *. rewrite map_length in H0. omega.
+    Qed.
+    Hint Resolve env_nil_by_length_eq : env_resolution.
+
+    Lemma all2_tvar_seq_dec_true : forall a b,
+      Folds.all2 Expr.tvar_seqb a b = true -> a = b.
+    Proof.
+      clear; induction a; destruct b; simpl; intros; try congruence.
+      consider (tvar_seqb a t). intros. erewrite IHa; auto.
+    Qed.
+
+    Lemma sym_evalStream_quant_append : forall path facts qs uvars vars ss res,
+      sym_evalStream Prover meval learnHook facts path qs uvars vars ss = res ->
+      match res with
+        | Safe qs' _ 
+        | SafeUntil qs' _ _ => exists qs'', qs' = appendQ qs'' qs
+(*        | Unsafe qs'  *)
+      end.
+    Proof.
+      clear.
+      induction path; simpl; intros.
+      { inversion H. subst. exists QBase.
+        clear. simpl; auto. }
+      { destruct a. destruct p. consider (sym_evalInstrs Prover meval facts l ss); intros; try congruence.
+        eapply IHpath; eauto. destruct p. subst. exists QBase. auto.
+        destruct s. destruct o. consider (sym_assertTest Prover meval facts s t s0 ss b); intros.
+        repeat match goal with 
+                 | [ H : match ?X with (_,_) => _ end = _ |- _ ] => destruct X; try congruence
+               end.
+        eapply IHpath in H0. destruct res; auto; destruct H0; rewrite <- appendQ_assoc in H0; eauto.
+        subst; auto. exists QBase; auto.        
+        repeat match goal with 
+                 | [ H : match ?X with _ => _ end = _ |- _ ] => destruct X; try congruence
+               end; subst;
+        try eapply IHpath; eauto.
+        exists QBase; auto.
+        exists QBase; auto. }
+    Qed.
+
+    Lemma typeof_env_app : forall ts a b,
+      typeof_env (types := ts) (a ++ b) = typeof_env a ++ typeof_env b.
+    Proof.
+      clear. unfold typeof_env. intros. rewrite map_app. reflexivity.
+    Qed.
+
+    Hint Extern 1 (@eq (list tvar) _ _) =>
+      simpl; repeat (rewrite app_nil_r in * || rewrite typeof_env_app in * || rewrite app_ass || 
+        (f_equal; []) || (f_equal; [ solve [ reflexivity | assumption ] | ] || reflexivity || assumption)) : env_resolution.
+      
+    Definition NO_MORE_COND : Prop := True.
+
+    Ltac sym_eval_prover IHpath := 
+      repeat match goal with
+               | [ H : Valid _ (?A ++ ?b) (?C ++ ?d) _
+                 , H' : sym_instrsD ?X ?A ?C ?Y = ?Z |- _ ] =>
+                 apply sym_instrsD_weaken with (B := b) (D := d) in H'
+               | [ H : Valid _ (?A ++ ?b) (?C ++ ?d) _
+                 , H' : istreamD ?X ?A ?C ?Y ?Z ?P ?L |- _ ] =>
+                 apply istreamD_weaken with (B := b) (D := d) in H'
+               | [ H : (_,_) = (_,_) |- _ ] => inversion H; clear H; subst
                | [ H : Some _ = Some _ |- _ ] => inversion H; clear H; subst
-             end; subst; eauto.
-    t_correct. destruct a; t_correct.
-        Focus.
-          eapply sym_evalInstrs_correct in H; eauto. simpl in *.
-          rewrite H4 in *.
-          revert H; case_eq (sym_evalInstrs Prover meval facts l ss); intros.
-          specialize (IHpath _ _ H5 _ _ H2 _ H1); eauto.
-          destruct p. simpl. destruct (sym_instrsD l1); try congruence.
-          destruct H2. destruct sound_or_safe; intuition eauto. contradiction.
+               | [ H : Safe _ _ = Safe _ _ |- _ ] => inversion H; clear H; subst
+               | [ H : SafeUntil _ _ _ = SafeUntil _ _ _ |- _ ] => inversion H; clear H; subst
+               | [ H : inl _ = inl _ |- _ ] => inversion H; clear H; subst
+               | [ H : inr _ = inr _ |- _ ] => inversion H; clear H; subst
+               | [ H : SymAssertCond _ _ _ _ = SymAssertCond _ _ _ _ |- _ ] => inversion H; clear H; subst
+               | [ H : sum (prod _ _) _ |- _ ] => destruct H as [ [ ? ? ] | ? ]
+               | [ H : ?X = _ , H' : ?X = _ |- _ ] => rewrite H in H'
+               | [ H : option state |- _ ] => destruct H
+               | [ H : _ /\ _ |- _ ] => destruct H
+               | [ H : ?X = _ , H' : context [ match ?X with _ => _ end ] |- _ ] =>
+                 rewrite H in H'
+               | [ H : match ?X with _ => _ end |- _ ] =>
+                 (revert H; case_eq X; intros; try contradiction); []
+               | [ |- _ ] => progress (repeat rewrite app_nil_r in * )
+               | [ |- _ ] => solve [ congruence | eauto with stateD_solver ]
+               | [ H : ?X -> _ , H' : ?X |- _ ] =>
+                 match type of X with
+                   | Prop => 
+                     specialize (H H')
+                 end
+               | [ H   : sym_evalInstrs _ _ ?F ?is ?S = _
+                 , H'  : evalInstrs ?stn ?st _ = _ 
+                 , H'' : sym_instrsD _ ?U ?G _ = Some ?isD
+                 , Hst : stateD _ _ _ _ _ _ _ 
+                 |- _ ] => 
+               ( eapply sym_evalInstrs_correct with (stn_st := (stn,st)) (facts := F) (ss := S) in H'' ; eauto ;
+                 simpl in H'' ) ; [ clear Hst ] 
+               | [ H : Structured.evalCond ?l ?A ?r ?B ?C = _ 
+                 , Hst : stateD _ _ ?U ?G ?cs _ _
+                 , H' : sym_rvalueD _ _ _ _ = Some ?l
+                 , H'' : sym_rvalueD _ _ _ _ = Some ?r |- _ ] =>
+               match goal with 
+                 | [ H : NO_MORE_COND |- _ ] => fail 1
+                 | _ =>
+                   (generalize Hst; eapply sym_assertTest_correct' with (meta_env := U) (vars_env := G) (t := A) (rD := l) (lD := r) (stn_st := (B,C)) in Hst; eauto using sym_rvalueD_weaken) ; [ intro; simpl in Hst ; assert NO_MORE_COND by (exact I) ]
+               end
+               | [ H : learnHook _ ?U' ?G' ?SS ?f ?F = (?A, ?B)
+                 , H' : stateD _ _ ?U ?G _ _ _ 
+                 , LC : MEVAL.LearnHook_correct _ _ _ _ 
+                 , PC : ProverT_correct _ _ |- _ ] =>
+                 (cutrewrite (U' = typeof_env U) in H; [ | rewrite typeof_env_app; f_equal; auto ] ;
+                  cutrewrite (G' = typeof_env G) in H; [ | rewrite typeof_env_app; f_equal; auto ] ;
+                  eapply (@MEVAL.hook_sound _ _ _ _ _ _ _ _ LC _ PC U G) with 
+                    (new_facts := F) (ss := SS) (ss' := A) (quant := B) in H ;
+                  eauto using Learn_correct, AllProvable_cons, AllProvable_nil with stateD_solver) ; [ clear H' ] 
+               | [ H : quantD _ _ _ _ |- quantD _ _ _ _ ] =>
+                 eapply quantD_impl; [ eapply H | clear H ; simpl; intros ]
+               | [ |- quantD _ _ (appendQ _ ?X) _ ] =>
+                 apply quantD_app
+               | [ H : appendQ _ _ = appendQ _ _ |- _ ] => apply appendQ_proper in H; subst
 
-        Focus.
-          eapply sym_evalInstrs_correct in H; eauto; simpl in *.
-          rewrite H3 in *.
-          destruct (sym_evalInstrs facts l ss); try contradiction.
-          destruct p. simpl. destruct (sym_instrsD l1); try contradiction.
-          destruct H; intuition; destruct sound_or_safe; eauto.
+               | [ H : appendQ ?A ?B = appendQ _ (appendQ _ ?B) |- _ ] => 
+                 rewrite <- appendQ_assoc in H; apply appendQ_proper in H; subst
+               | [ H : context [ Safe (appendQ (appendQ ?A ?B) ?C) _ ] |- _ ] =>
+                 rewrite appendQ_assoc with (a := A) (b := B) (c := C) in H
+               | [ H : context [ SafeUntil (appendQ (appendQ ?A ?B) ?C) _ _ ] |- _ ] =>
+                 rewrite appendQ_assoc with (a := A) (b := B) (c := C) in H
+                 
+               | [ H : sym_evalStream _ _ _ _ _ (appendQ _ ?X) _ _ _ = Safe (appendQ ?Y ?X) _ |- _ ] =>
+                 match Y with
+                   | appendQ _ _ => fail 1
+                   | _ => destruct (sym_evalStream_quant_append _ _ _ _ _ _ H); subst
+                 end
+               | [ H : sym_evalStream _ _ _ _ _ (appendQ _ (appendQ _ ?X)) _ _ _ = Safe (appendQ ?Y ?X) _ |- _ ] =>
+                 match Y with
+                   | appendQ _ _ => fail 1
+                   | _ => rewrite <- appendQ_assoc in H; destruct (sym_evalStream_quant_append _ _ _ _ _ _ H); subst
+                 end
+               | [ H : sym_evalStream _ _ _ _ _ (appendQ _ ?X) _ _ _ = SafeUntil (appendQ ?Y ?X) _ _ |- _ ] =>
+                 match Y with
+                   | appendQ _ _ => fail 1
+                   | _ => destruct (sym_evalStream_quant_append _ _ _ _ _ _ H); subst
+                 end
+               | [ H : sym_evalStream _ _ _ _ _ (appendQ _ (appendQ _ ?X)) _ _ _ = SafeUntil (appendQ ?Y ?X) _ _ |- _ ] =>
+                 match Y with
+                   | appendQ _ _ => fail 1
+                   | _ => rewrite <- appendQ_assoc in H; destruct (sym_evalStream_quant_append _ _ _ _ _ _ H); subst
+                 end
+               | [ H : EqNat.beq_nat ?X ?Y = true |- _ ] => 
+                 symmetry in H; apply EqNat.beq_nat_eq in H
+               | [ H : Folds.all2 _ _ _ = true |- _ ] => 
+                 eapply all2_tvar_seq_dec_true in H
+               | [ H : sym_evalStream _ _ _ _ _ ?QS _ _ _ = _ 
+                 , H' : stateD _ _ ?Uall ?Gall _ (_, ?st) _
+                 , H'' : istreamD _ _ _ _ _ ?st _
+                 |- _ ] =>
+               let t := change (QS) with (appendQ QBase QS) in H at 1 ; 
+                 eapply IHpath with (env_q := QS) (qs := QBase) (meta_env := Uall) (vars_env := Gall) in H;
+                   simpl; subst; intuition (eauto using istreamD_weaken, Valid_weaken with env_resolution) in
+               solve [ t ] || (t; [])
+               | [ H : forall res : bool, match sym_assertTest _ _ _ _ _ _ _ res with _ => _ end |- _ ] =>
+                 specialize (H true); unfold sym_assertTest in H
+               | [ H : match ?X with | IL.Eq => _ | _ => _ end = None |- _ ] =>
+                 destruct X; congruence
+               | [ H : exists x : state, _ |- exists y : state, _ ] => 
+                 let s := fresh "st" in 
+                 solve [ destruct H as [ s ? ] ; exists s ; intuition ]
+               | [ H : match ?X with _ => _ end |- _ ] =>
+                 (revert H; case_eq X; intros; try contradiction)
+               | [ H : match ?X with _ => _ end = _ |- _ ] =>
+                 (revert H; case_eq X; intros; try split_congruence)
+               | [ H : sym_rvalueD _ _ _ _ = _ |- context [ sym_rvalueD _ _ _ _ ] ] =>
+                   erewrite sym_rvalueD_weaken by eauto
+               | [ H : option bool |- _ ] => destruct H
+             end.
 
-        Focus.
-          destruct s. revert H.
-          case_eq (sym_rvalueD s); case_eq (sym_rvalueD s0); intros; try contradiction.
-          destruct o.
-          generalize (sym_assertTest_correct facts _ _ t _ _ _ H0 H2 H b).
-          simpl. destruct H3. rewrite H3.
-          case_eq (sym_assertTest facts s t s0 ss b); intros.
-          eapply IHpath; eauto.
-          
-          destruct 
-*)
-    Admitted.
+    Lemma evalStream_correct_Safe : forall sound_or_safe cs stn path facts ss qs qs' ss' uvars vars env_q,
+      sym_evalStream Prover meval learnHook facts path (appendQ qs env_q) uvars vars ss = Safe (appendQ qs' env_q) ss' ->
+      forall meta_env vars_env,
+        typeof_env meta_env ++ gatherAll qs = uvars ->
+        typeof_env vars_env ++ gatherEx qs = vars ->
+        forall st,
+          istreamD funcs meta_env vars_env path stn st sound_or_safe ->
+        quantD vars_env meta_env qs (fun vars_env meta_env =>
+          stateD funcs preds meta_env vars_env cs (stn,st) ss /\
+          Valid PC meta_env vars_env facts) ->
+        quantD vars_env meta_env qs' (fun vars_env meta_env =>
+          match sound_or_safe with
+            | None => False
+            | Some (st') =>
+              stateD funcs preds meta_env vars_env cs (stn, st') ss'
+          end).
+    Proof.
+      Opaque stateD. 
+      induction path; simpl; intros; sym_eval_prover IHpath; try contradiction.
+    Qed.
+
+    Lemma evalStream_correct_SafeUntil : forall sound_or_safe cs stn path facts ss qs qs' ss' is' uvars vars env_q,
+      sym_evalStream Prover meval learnHook facts path (appendQ qs env_q) uvars vars ss = SafeUntil (appendQ qs' env_q) ss' is' ->
+      forall meta_env vars_env,
+        typeof_env meta_env ++ gatherAll qs = uvars ->
+        typeof_env vars_env ++ gatherEx qs = vars ->
+        forall st,
+          istreamD funcs meta_env vars_env path stn st sound_or_safe ->
+        quantD vars_env meta_env qs (fun vars_env meta_env =>
+          stateD funcs preds meta_env vars_env cs (stn,st) ss /\
+          Valid PC meta_env vars_env facts) ->
+        quantD vars_env meta_env qs' (fun vars_env meta_env =>
+          exists st' : state,
+          stateD funcs preds meta_env vars_env cs (stn, st') ss' /\
+          istreamD funcs meta_env vars_env is' stn st' sound_or_safe).
+    Proof.
+      induction path; simpl; intros; sym_eval_prover IHpath; try contradiction. 
+    Qed.
+
+    Lemma appendQ_QBase_r : forall a, appendQ a QBase = a.
+    Proof. clear. induction a; simpl; intros; think; auto. Qed.
+
+    Theorem evalStream_correct : forall sound_or_safe cs stn path facts ss qs uvars vars res,
+      sym_evalStream Prover meval learnHook facts path qs uvars vars ss = res ->
+      forall meta_env vars_env,
+        typeof_env meta_env ++ gatherAll qs = uvars ->
+        typeof_env vars_env ++ gatherEx qs = vars ->
+        forall st,
+          istreamD funcs meta_env vars_env path stn st sound_or_safe ->
+        quantD vars_env meta_env qs (fun vars_env meta_env =>
+          stateD funcs preds meta_env vars_env cs (stn,st) ss /\
+          Valid PC meta_env vars_env facts) ->
+        match res with
+          | Safe qs' ss' =>
+            quantD vars_env meta_env qs' (fun vars_env meta_env =>
+              match sound_or_safe with
+                | None => False
+                | Some (st') => stateD funcs preds meta_env vars_env cs (stn, st') ss'
+              end)
+          | SafeUntil qs' ss' is' =>
+            quantD vars_env meta_env qs' (fun vars_env meta_env =>
+              exists st' : state,
+                stateD funcs preds meta_env vars_env cs (stn, st') ss' /\
+                istreamD funcs meta_env vars_env is' stn st' sound_or_safe)
+        end.
+    Proof.
+      destruct res; intros.
+      { destruct (sym_evalStream_quant_append _ _ _ _ _ _ H).
+        generalize (@evalStream_correct_Safe sound_or_safe cs stn path facts ss qs (appendQ x qs) s uvars vars QBase). subst.
+        repeat rewrite appendQ_QBase_r. intro. eapply H0 in H; eauto. }
+      { destruct (sym_evalStream_quant_append _ _ _ _ _ _ H).
+        generalize (@evalStream_correct_SafeUntil sound_or_safe cs stn path facts ss qs (appendQ x qs) s i uvars vars QBase); 
+          subst.
+        repeat rewrite appendQ_QBase_r. intro. eapply H0 in H; eauto. }
+    Qed.
   End typed2.
 
-
-(*
-  Section iface.
-    Variable ts : list type.
-    Let types := repr bedrock_types_r ts.
-
-    Local Notation "'pcT'" := (tvType 0).
-    Local Notation "'tvWord'" := (tvType 0).
-    Local Notation "'stT'" := (tvType 1).
-    Local Notation "'tvState'" := (tvType 2).
-    Local Notation "'tvTest'" := (tvType 3).
-    Local Notation "'tvReg'" := (tvType 4).
-
-    Theorem sym_evalInstr_correct : 
-      forall (fs : functions types) (preds : SEP.predicates types (tvType 0) (tvType 1)),
-        let funcs := repr (bedrock_funcs_r ts) fs in
-        forall (Prover : ProverT types) (PC : ProverT_correct Prover funcs)
-          (meval : MEVAL.MemEvaluator types (tvType 0) (tvType 1))
-          (meval_correct : MEVAL.MemEvaluator_correct meval funcs preds (tvType 0) (tvType 0)
-            (@IL_mem_satisfies ts) (@IL_ReadWord ts) (@IL_WriteWord ts)),
-      
-        forall (facts : Facts Prover) (meta_env var_env : env types) instr stn_st instrD cs ss ss',
-        Valid PC meta_env var_env facts  ->
-        stateD funcs preds meta_env var_env cs stn_st ss ->
-        sym_instrD funcs meta_env var_env instr = Some instrD ->
-        sym_evalInstr Prover meval facts instr ss = Some ss' ->
-        exists st',
-          evalInstr (fst stn_st) (snd stn_st) instrD = Some st' /\
-          stateD funcs preds meta_env var_env cs (fst stn_st, st') ss'.
-    Proof.
-      intros. eapply sym_evalInstr_correct'; eauto.
-    Qed.
-
-    Theorem sym_assertTest_correct : 
-      forall (fs : functions types) (preds : SEP.predicates types (tvType 0) (tvType 1)),
-        let funcs := repr (bedrock_funcs_r ts) fs in
-        forall (Prover : ProverT types) (PC : ProverT_correct Prover funcs)
-          (meval : MEVAL.MemEvaluator types (tvType 0) (tvType 1))
-          (meval_correct : MEVAL.MemEvaluator_correct meval funcs preds (tvType 0) (tvType 0)
-            (@IL_mem_satisfies ts) (@IL_ReadWord ts) (@IL_WriteWord ts)),
-          forall (facts : Facts Prover) (meta_env var_env : env types) cs r rD t l lD ss stn_st,
-            Valid PC meta_env var_env facts  ->
-            stateD funcs preds meta_env var_env cs stn_st ss ->
-            sym_rvalueD funcs meta_env var_env r = Some rD ->
-            sym_rvalueD funcs meta_env var_env l = Some lD ->
-              match Structured.evalCond rD t lD (fst stn_st) (snd stn_st) with
-                | None =>
-                  forall res, 
-                    match sym_assertTest Prover meval facts r t l ss res with
-                      | Some _ => False
-                      | None => True
-                    end
-                | Some res' =>
-                  match sym_assertTest Prover meval facts r t l ss res' with
-                    | Some b => 
-                      Provable funcs meta_env var_env b
-                    | None => True
-                  end
-              end.
-    Proof.
-      intros; eapply sym_assertTest_correct'; eauto.
-    Qed.
-  End iface.
-*)
-
 End SymIL_Correct.
-
